rearranged code and went through CompileModule.v

platform/cito/SepHints5.v
@@ -10,3 +10,42 @@ Definition hints_split_buf : TacPackage.
   prepare split_buf tt.
 Defined.
 
+Definition to_intro_array (_ : W) := True.
+
+Lemma intro_array : forall len p, to_intro_array p -> p =?> len ===> Ex ls, [| length ls = len |] * array ls p.
+  admit.
+Qed.
+
+Definition combined_locals vars1 vars2 vs1 vs2 p  := locals (vars1 ++ vars2) (merge vs1 vs2 vars1) 0 p.
+
+Lemma fold_combined_locals : forall vars1 vars2 vs1 vs2 p, locals (vars1 ++ vars2) (merge vs1 vs2 vars1) 0 p = combined_locals vars1 vars2 vs1 vs2 p.
+  eauto.
+Qed.
+
+Definition locals_combinable A (vars vars2 : list A) := NoDup (vars ++ vars2).
+
+Lemma combine_locals : forall vars1 vars2 vs1 vs2 p, locals vars1 vs1 0 p * locals vars2 vs2 0 (p ^+ $(4 * length vars1)) ===> combined_locals vars1 vars2 vs1 vs2 p.
+  admit.
+Qed.
+
+Definition hints_intro_array : TacPackage.
+  prepare intro_array tt.
+Defined.
+
+Definition hints_combine_locals : TacPackage.
+  prepare tt combine_locals.
+Defined.
+
+Definition locals_to_split vars1 vars2 vs p := locals (vars1 ++ vars2) vs 0 p.
+
+Lemma fold_locals_to_split : forall vars1 vars2 vs p, locals (vars1 ++ vars2) vs 0 p = locals_to_split vars1 vars2 vs p.
+  eauto.
+Qed.
+
+Lemma split_locals : forall vars1 vars2 vs p, locals_to_split vars1 vars2 vs p ===> locals vars1 vs 0 p * locals vars2 vs 0 (p ^+ $(4 * length vars1)).
+  admit.
+Qed.
+
+Definition hints_split_locals : TacPackage.
+  prepare split_locals tt.
+Defined.
